globals_lemmas

floyd/globals_lemmas.v
@@ -10,32 +10,7 @@ Require Import VST.floyd.data_at_list_solver.
 Require Import VST.floyd.closed_lemmas.
 Require Import VST.floyd.nested_pred_lemmas.
 Import LiftNotation.
-Import compcert.lib.Maps.
-Local Open Scope logic.
-
-Fixpoint fold_right_sepcon' (l: list(environ->mpred)) : environ -> mpred :=
- match l with
- | nil => emp
- | b::nil => b
- | b::r => b * fold_right_sepcon' r
- end.
-
-Lemma fold_right_sepcon'_eq:
-  fold_right_sepcon' = @fold_right (environ->mpred) _ sepcon emp.
-Proof.
-extensionality l rho.
-induction l; auto.
-simpl.
-destruct l. simpl. rewrite sepcon_emp. auto.
-f_equal; auto.
-Qed.
-
-
-Lemma orp_dup {A}{ND: NatDed A}: forall P: A, P || P = P.
-Proof. intros. apply pred_ext.
-apply orp_left; apply derives_refl.
-apply orp_right1; apply derives_refl.
-Qed.
+Import -(notations) compcert.lib.Maps.
 
 Lemma unsigned_repr_range: forall i, 0 <= i -> 0 <= Ptrofs.unsigned (Ptrofs.repr i) <= i.
 Proof.
@@ -52,14 +27,18 @@ Proof.
   (compute in x; subst x; spec H0; [lia| ]; spec H1; lia).
 Qed.
 
+Section mpred.
+
+Context `{!heapGS Σ}.
+
 Lemma tc_globalvar_sound:
   forall Delta i t gz idata rho,
-   (var_types Delta) ! i = None ->
-   (glob_types Delta) ! i = Some t ->
+   (var_types Delta) !! i = None ->
+   (glob_types Delta) !! i = Some t ->
    gvar_volatile gz = false ->
    gvar_init gz = idata ->
    tc_environ Delta rho ->
-   globvar2pred (globals_of_env rho) (i, gz) |-- init_data_list2pred (globals_of_env rho) idata (readonly2share (gvar_readonly gz)) (eval_var i t rho).
+   globvar2pred (globals_of_env rho) (i, gz) ⊢ init_data_list2pred (globals_of_env rho) idata (readonly2share (gvar_readonly gz)) (eval_var i t rho).
 Proof.
 intros.
 unfold globvar2pred.
@@ -69,18 +48,17 @@ destruct_var_types i.
 destruct_glob_types i.
 unfold globals_of_env.
 unfold eval_var.
-rewrite Heqo0, Heqo1, H1, H2.
-auto.
+rewrite Heqo0 Heqo1 H1 H2 //.
 Qed.
 
 Lemma tc_globalvar_sound':
   forall Delta i t gv idata rho,
-   (var_types Delta) ! i = None ->
-   (glob_types Delta) ! i = Some t ->
+   (var_types Delta) !! i = None ->
+   (glob_types Delta) !! i = Some t ->
    gvar_volatile gv = false ->
    gvar_init gv = idata ->
    tc_environ Delta rho ->
-   globvar2pred (globals_of_env rho) (i, gv) |--
+   globvar2pred (globals_of_env rho) (i, gv) ⊢
    init_data_list2pred (globals_of_env rho) idata (readonly2share (gvar_readonly gv)) (globals_of_env rho i).
 Proof.
 intros.
@@ -89,8 +67,7 @@ simpl.
 red in H3.
 destruct_glob_types i.
 unfold globals_of_env.
-rewrite Heqo0, H1, H2.
-auto.
+rewrite Heqo0 H1 H2 //.
 Qed.
 
 Definition zero_of_type (t: type) : val :=
@@ -117,12 +94,12 @@ Definition init_data2pred'
   | Init_float64 r =>  mapsto sh tdouble v (Vfloat r)
   | Init_space n =>  mapsto_zeros n sh v
   | Init_addrof symb ofs =>
-      match (var_types Delta) ! symb, (glob_types Delta) ! symb with
+      match (var_types Delta) !! symb, (glob_types Delta) !! symb with
       | None, Some (Tarray t n' att) =>
            mapsto sh (Tpointer t noattr) v (offset_val (Ptrofs.unsigned ofs) (gv symb))
       | None, Some t => mapsto sh (Tpointer t noattr) v (offset_val (Ptrofs.unsigned ofs) (gv symb))
       | Some _, Some _ => mapsto_ sh (Tpointer Tvoid noattr) v
-      | _, _ => TT
+      | _, _ => True
       end
  end.
 
@@ -139,26 +116,23 @@ Lemma mapsto_aligned:
  forall t ch, access_mode t = By_value ch ->
   forall  sh b z p,
   mapsto sh t (Vptr b z) p
-   |-- !! (Memdata.align_chunk ch | Ptrofs.unsigned z).
+   ⊢ ⌜(Memdata.align_chunk ch | Ptrofs.unsigned z)⌝.
 Proof.
 intros.
 unfold mapsto. simpl.
 rewrite H.
 if_tac.
-simple_if_tac.
-apply FF_left.
-apply orp_left. normalize. clear H H0.
-rewrite (res_predicates.address_mapsto_align).
-match goal with |- ?A |-- ?B => constructor; change (predicates_hered.derives A B) end.
-intros ? ?. destruct H. apply H0.
-normalize.
-clear.
-rewrite (res_predicates.address_mapsto_align).
-match goal with |- ?A |-- ?B => constructor; change (predicates_hered.derives A B) end.
-intros ? ?. destruct H. apply H0.
-simple_if_tac.
-apply FF_left.
-normalize.
+- simple_if_tac.
+  { iIntros "[]". }
+  iIntros "[H | H]".
+  + rewrite (res_predicates.address_mapsto_align).
+    iDestruct "H" as "(_ & _ & $)".
+  + iDestruct "H" as (??) "H".
+    rewrite (res_predicates.address_mapsto_align).
+    iDestruct "H" as "(_ & $)".
+- simple_if_tac.
+  { iIntros "[]". }
+  normalize.
 Qed.
 
 Lemma sizeof_Tpointer {cs: compspecs} : forall t, 
@@ -182,7 +156,7 @@ Lemma init_data2pred_rejigger {cs: compspecs}:
   v = Vptr b (Ptrofs.repr 0) ->
   readable_share sh ->
    init_data2pred (globals_of_env rho) idata sh (offset_val ofs v)
-    |-- init_data2pred' Delta (globals_of_env rho) idata sh (offset_val ofs v).
+    ⊢ init_data2pred' Delta (globals_of_env rho) idata sh (offset_val ofs v).
 Proof.
 intros until v.
 intros H7 H8 RS.
@@ -196,24 +170,23 @@ assert (H6:=I).
  destruct idata; super_unfold_lift; try apply derives_refl.
  red in H7.
  unfold globals_of_env.
- destruct_var_types i eqn:Hv&Hv'; rewrite ?Hv, ?Hv';
-  destruct_glob_types i eqn:Hg&Hg'; rewrite ?Hg, ?Hg';
+ destruct_var_types i eqn:Hv&Hv'; rewrite ?Hv ?Hv';
+  destruct_glob_types i eqn:Hg&Hg'; rewrite ?Hg ?Hg';
 try solve [simpl; apply TT_right].
  + rewrite H8. cancel.
  + replace (offset_val (Ptrofs.unsigned i0) (globals_of_env rho i)) with (Vptr b0 i0).
-   replace (mapsto sh (Tpointer Tvoid noattr) (offset_val ofs v) (Vptr b0 i0))
-   with (mapsto sh (Tpointer t noattr) (offset_val ofs v) (Vptr b0 i0)).
-   simpl offset_val. rewrite !Ptrofs.add_zero_l.
-   rewrite Ptrofs.repr_unsigned.
-   destruct t; auto; try apply derives_refl.
+   trans (mapsto sh (Tpointer t noattr) (offset_val ofs v) (Vptr b0 i0)).
+   2: { simpl offset_val. rewrite !Ptrofs.add_zero_l.
+        rewrite Ptrofs.repr_unsigned.
+        destruct t; auto; try apply derives_refl.
+        unfold mapsto; simpl.
+        destruct (offset_val ofs v); auto. rewrite -> !if_true by auto. rewrite andb_false_r.
+        apply derives_refl. }
    unfold mapsto; simpl.
-   destruct (offset_val ofs v); auto. rewrite !if_true by auto. rewrite andb_false_r.
-   apply derives_refl.
-   unfold mapsto; simpl.
-   destruct (offset_val ofs v); auto. rewrite !if_true by auto. rewrite andb_false_r.
-   reflexivity.
-   unfold globals_of_env. rewrite Hg'. simpl. rewrite Ptrofs.add_zero_l.
-   f_equal. rewrite Ptrofs.repr_unsigned; auto.
+   destruct (offset_val ofs v); auto. rewrite andb_false_r /=. rewrite -> !if_true by auto.
+   rewrite !Ptrofs.add_zero_l //.
+   { unfold globals_of_env. rewrite Hg'. simpl. rewrite Ptrofs.add_zero_l.
+     f_equal. rewrite Ptrofs.repr_unsigned; auto. }
 Qed.
 
 Lemma readable_readonly2share: forall ro, readable_share (readonly2share ro).
@@ -223,49 +196,47 @@ Qed.
 
 Lemma unpack_globvar  {cs: compspecs}:
   forall Delta gz i t gv idata,
-   (var_types Delta) ! i = None ->
-   (glob_types Delta) ! i = Some t ->
+   (var_types Delta) !! i = None ->
+   (glob_types Delta) !! i = Some t ->
   (complete_legal_cosu_type (gvar_info gv) && is_aligned cenv_cs ha_env_cs la_env_cs (gvar_info gv) 0 = true)%bool ->
    gvar_volatile gv = false ->
    gvar_info gv = t ->
    gvar_init gv = idata :: nil ->
    init_data_size idata <= sizeof t ->
    sizeof t <= Ptrofs.max_unsigned ->
-   local (`and (tc_environ Delta) (fun rho =>gz = globals_of_env rho)) && `(globvar2pred gz (i, gv)) |--
-       `(init_data2pred' Delta gz idata (readonly2share (gvar_readonly gv)) (gz i)).
+   local (`and (tc_environ Delta) (fun rho =>gz = globals_of_env rho)) ∧ ⎡globvar2pred gz (i, gv)⎤ ⊢
+       ⎡init_data2pred' Delta gz idata (readonly2share (gvar_readonly gv)) (gz i)⎤.
 Proof.
 intros.
 go_lowerx. subst gz.
-eapply derives_trans; [eapply tc_globalvar_sound'; try eassumption | ].
+etrans; [eapply tc_globalvar_sound'; try eassumption | ].
 assert (RS:= readable_readonly2share (gvar_readonly gv)).
 forget (readonly2share (gvar_readonly gv)) as sh.
 autorewrite with subst norm1 norm2; normalize.
 unfold init_data_list2pred.
-rewrite sepcon_emp.
+rewrite bi.sep_emp.
 destruct (globvar_eval_var _ _ _ _ H7 H H0) as [b [? ?]].
 assert (globals_of_env rho i = offset_val 0 (globals_of_env rho i)).
 unfold globals_of_env.
 rewrite H9. reflexivity.
-rewrite H10 at 1.
- apply derives_trans with
-     (init_data2pred' Delta (globals_of_env rho) idata sh
+rewrite -> H10 at 1.
+trans (init_data2pred' Delta (globals_of_env rho) idata sh
       (offset_val 0 (globals_of_env rho i))).
 + rewrite andb_true_iff in H1; destruct H1.
   eapply init_data2pred_rejigger; eauto; try lia.
   unfold globals_of_env; rewrite H9; reflexivity.
- +
- unfold init_data2pred'.
++ unfold init_data2pred'.
   rewrite <- H10.
- destruct idata; unfold_lift;
-   try (rewrite H8; simpl; rewrite Ptrofs.add_zero_l; auto);
- try apply derives_refl.
+  destruct idata; unfold_lift;
+    try (rewrite H8; simpl; rewrite Ptrofs.add_zero_l; auto);
+  try apply derives_refl.
 Qed.
 
 Fixpoint id2pred_star   {cs: compspecs}
    (Delta: tycontext) (gz: globals) (sh: share) (v: val) (dl: list init_data) : mpred :=
  match dl with
  | d::dl' => init_data2pred' Delta gz d sh v
-                   * id2pred_star Delta gz sh (offset_val (init_data_size d) v) dl'
+                   ∗ id2pred_star Delta gz sh (offset_val (init_data_size d) v) dl'
  | nil => emp
  end.
 
@@ -286,48 +257,38 @@ Qed.
 
 Lemma unpack_globvar_star  {cs: compspecs}:
   forall Delta gz i gv,
-   (var_types Delta) ! i = None ->
-   (glob_types Delta) ! i = Some (gvar_info gv) ->
+   (var_types Delta) !! i = None ->
+   (glob_types Delta) !! i = Some (gvar_info gv) ->
    gvar_volatile gv = false ->
-   local (`and (tc_environ Delta) (fun rho =>gz = globals_of_env rho)) && `(globvar2pred gz (i, gv)) |-- 
-       `(id2pred_star Delta gz (readonly2share (gvar_readonly gv)) (gz i) (gvar_init gv)).
+   local (`and (tc_environ Delta) (fun rho =>gz = globals_of_env rho)) ∧ ⎡globvar2pred gz (i, gv)⎤ ⊢
+       ⎡id2pred_star Delta gz (readonly2share (gvar_readonly gv)) (gz i) (gvar_init gv)⎤.
 Proof.
 intros until 2. pose proof I. intros H2.
-pose (H5 := True).
 remember (gvar_info gv) as t eqn:H3; symmetry in H3.
 remember (gvar_init gv) as idata eqn:H4; symmetry in H4.
 intros.
-pose (H6:=True).
-go_lowerx. subst gz.
-eapply derives_trans; [eapply tc_globalvar_sound'; eassumption | ].
-normalize.
-  autorewrite with subst norm1 norm2; normalize.
-match goal with |- _ |-- ?F _ _ _ _ _ _  => change F with @id2pred_star end.
-normalize.
-  autorewrite with subst norm1 norm2; normalize.
+go_lowerx. fold id2pred_star. subst gz.
+etrans; [eapply tc_globalvar_sound'; eassumption | ].
 assert (RS:= readable_readonly2share (gvar_readonly gv)).
 forget (readonly2share (gvar_readonly gv)) as sh.
 set (ofs:=0%Z).
 assert (alignof t | Ptrofs.unsigned (Ptrofs.repr ofs)) by (subst ofs; simpl; apply Z.divide_0_r).
-destruct (globvar_eval_var _ _ _ _ H7 H H0) as [b [_ H9']].
+destruct (globvar_eval_var _ _ _ _ H5 H H0) as [b [_ H9']].
 unfold globals_of_env. rewrite H9'. clear H9'.
 remember (Vptr b Ptrofs.zero) as x.
 replace x with (offset_val ofs x) at 1 2 by (subst x; normalize).
 fold (globals_of_env rho).
 clearbody ofs.
-clear H1 H8 gv H3 H2 H4 H H0 H6 H5.
+clear - H5 RS Heqx.
 revert ofs.
 induction idata; simpl; auto; intros.
-match goal with |- _ |-- _ * ?F _ _ _ _ _ _  => 
-    change F with @id2pred_star 
-end.
-apply sepcon_derives.
-*
-  clear IHidata. 
+fold id2pred_star.
+apply bi.sep_mono.
+* clear IHidata.
   eapply init_data2pred_rejigger; eauto.
 * specialize (IHidata (ofs + init_data_size a)).
-   rewrite offset_offset_val.
- apply IHidata.
+  rewrite offset_offset_val.
+  apply IHidata.
 Qed.
 
 Definition inttype2init_data (sz: intsize) : (int -> init_data) :=
@@ -346,30 +307,30 @@ Lemma id2pred_star_ZnthV_Tint  {cs: compspecs} :
   (NBS: notboolsize sz),
   n = Zlength mdata ->
   mdata = map (inttype2init_data sz) data ->
-  !! isptr v && !! align_compatible (Tint sz sign noattr) v &&
-  !! (offset_strict_in_range (sizeof (Tint sz sign noattr) * n)) v &&
-  `(id2pred_star Delta gz sh v mdata) |--
-  `(data_at sh (tarray (Tint sz sign noattr) n)
-           (map (Basics.compose Vint (Cop.cast_int_int sz sign)) data) v).
+  ⌜isptr v⌝ ∧ ⌜align_compatible (Tint sz sign noattr) v⌝ ∧
+  ⌜offset_strict_in_range (sizeof (Tint sz sign noattr) * n) v⌝ ∧
+  (⎡id2pred_star Delta gz sh v mdata⎤ : assert) ⊢
+  ⎡data_at sh (tarray (Tint sz sign noattr) n)
+           (map (Basics.compose Vint (Cop.cast_int_int sz sign)) data) v⎤.
 Proof.
   intros. subst n mdata.
   replace (Zlength (map  (inttype2init_data sz) data)) with (Zlength data)
     by (repeat rewrite Zlength_correct; rewrite map_length; auto).
   go_lowerx.
-  match goal with |- ?F _ _ _ _ _ _ |-- _ => change F with @id2pred_star end.
+  fold id2pred_star.
   change (offset_strict_in_range (sizeof (Tint sz sign noattr) * Zlength data) v) in H1.
   assert (offset_strict_in_range (sizeof (Tint sz sign noattr) * 0) v) by
     (unfold offset_strict_in_range; destruct v; auto; pose proof Ptrofs.unsigned_range i; lia).
-unfold tarray.
-set (t := Tint sz sign noattr) in *.
-revert v H H0 H1 H2; induction data; intros.
+  unfold tarray.
+  set (t := Tint sz sign noattr) in *.
+  revert v H H0 H1 H2; induction data; intros.
 *
   rewrite Zlength_nil. unfold data_at, field_at; simpl.
   unfold at_offset; simpl.
    unfold nested_field_type; simpl.
    rewrite data_at_rec_eq. unfold  aggregate_pred.aggregate_pred.array_pred.
   unfold aggregate_pred.array_pred. simpl.
-  repeat apply andp_right; auto; try apply prop_right; try reflexivity.  
+  repeat apply bi.and_intro; auto; try apply bi.pure_intro; try reflexivity.
   hnf. simpl.
   split3; auto.
   split3; auto.
@@ -385,11 +346,11 @@ erewrite (split2_data_at_Tarray sh t (Z.succ (Zlength data)) 1).
 4: apply eq_refl.
 2: list_solve.
 2: list_solve. 2: auto. 2: list_solve. 2: apply eq_refl. 2: apply eq_refl.
-rewrite (sublist_one) by list_solve.
+rewrite -> (sublist_one) by list_solve.
 autorewrite with sublist.
 rewrite sublist_1_cons.
-rewrite sublist_same by list_solve.
-apply sepcon_derives.
+rewrite -> sublist_same by list_solve.
+apply bi.sep_mono.
 +
 clear IHdata.
 fold (tarray t 1). erewrite data_at_singleton_array_eq by apply eq_refl.
@@ -429,14 +390,14 @@ apply derives_refl.
    destruct v; try contradiction.
    pose proof (Ptrofs.unsigned_range i).
    assert (Ptrofs.max_unsigned = Ptrofs.modulus-1) by computable.
-   rewrite Z.mul_0_r in *.
+   rewrite -> Z.mul_0_r in *.
    assert (0 <= sizeof t * Zlength data) by (apply Z.mul_nonneg_nonneg; lia).
    unfold offset_strict_in_range, offset_val in *.
    unfold align_compatible in H0|-*.
    unfold Ptrofs.add.
-   rewrite (Ptrofs.unsigned_repr (sizeof t)) 
+   rewrite -> (Ptrofs.unsigned_repr (sizeof t)) 
     by (unfold sizeof, Ptrofs.max_unsigned, Ptrofs.modulus, Ptrofs.wordsize, Wordsize_Ptrofs.wordsize;
-          clear; subst t; destruct sz,sign, Archi.ptr64; simpl; lia).
+          clear; subst t; destruct sz,sign, Archi.ptr64; simpl; computable).
   rewrite Ptrofs.unsigned_repr.
   split3; try lia.
    assert (exists ch, access_mode t = By_value ch)
@@ -450,10 +411,10 @@ apply derives_refl.
   lia.
  }
  destruct H8 as [H8a [H8b H8c]].
-  eapply derives_trans; [ apply IHdata | ]; clear IHdata; auto.
+  etrans; [ apply IHdata | ]; clear IHdata; auto.
   replace (Z.succ (Zlength data) - 1) with (Zlength data) by (clear; lia).
-   apply derives_refl'; f_equal.
- unfold field_address0.
+  apply bi.equiv_entails_1_1; f_equiv; hnf.
+  unfold field_address0.
   rewrite if_true.
   unfold offset_val. destruct v; simpl; auto. f_equal.
   subst t; destruct sz,sign; reflexivity.
@@ -464,7 +425,7 @@ apply derives_refl.
   split3; auto; red.
   unfold sizeof, Ctypes.sizeof;  fold Ctypes.sizeof. fold (sizeof t).
   pose proof (Zlength_nonneg data).
-  rewrite Z.max_r by lia.
+  rewrite -> Z.max_r by lia.
   unfold offset_strict_in_range in H1. rewrite Zlength_cons in H1.
   lia.
   apply align_compatible_rec_Tarray; intros.
@@ -487,10 +448,10 @@ Lemma id2pred_star_ZnthV_tint  {cs: compspecs}:
  forall Delta gz sh n (v: val) (data: list int) mdata,
   n = Zlength mdata ->
   mdata = map Init_int32 data ->
-  !! isptr v && !! align_compatible tint v &&
-  !! offset_strict_in_range (sizeof tint * n) v &&
-  `(id2pred_star Delta gz sh v mdata) |--
-  `(data_at sh (tarray tint n) (map Vint data) v).
+  ⌜isptr v⌝ ∧ ⌜align_compatible tint v⌝ ∧
+  ⌜offset_strict_in_range (sizeof tint * n) v⌝ ∧
+  (⎡id2pred_star Delta gz sh v mdata⎤ : assert) ⊢
+  ⎡data_at sh (tarray tint n) (map Vint data) v⎤.
 Proof. intros; apply id2pred_star_ZnthV_Tint; auto; apply Coq.Init.Logic.I.
 Qed.
 
@@ -504,8 +465,8 @@ Qed.
 
 Lemma unpack_globvar_array  {cs: compspecs}:
   forall t sz sign (data: list int)  n Delta gz i gv,
-   (var_types Delta) ! i = None ->
-   (glob_types Delta) ! i = Some (gvar_info gv) ->
+   (var_types Delta) !! i = None ->
+   (glob_types Delta) !! i = Some (gvar_info gv) ->
    gvar_info gv = tarray t n ->
    gvar_volatile gv = false ->
    t = Tint sz sign noattr ->
@@ -513,44 +474,24 @@ Lemma unpack_globvar_array  {cs: compspecs}:
    n = Zlength (gvar_init gv) ->
    gvar_init gv = map (inttype2init_data sz) data ->
    init_data_list_size (gvar_init gv) <= sizeof (gvar_info gv) <= Ptrofs.max_unsigned ->
-   local (`and (tc_environ Delta) (fun rho =>gz = globals_of_env rho)) && `(globvar2pred gz(i, gv)) |--
-      `(data_at (readonly2share (gvar_readonly gv))
+   local (`and (tc_environ Delta) (fun rho =>gz = globals_of_env rho)) ∧ ⎡globvar2pred gz(i, gv)⎤ ⊢
+      ⎡data_at (readonly2share (gvar_readonly gv))
          (tarray (Tint sz sign noattr) n)
          (map (Basics.compose Vint (Cop.cast_int_int sz sign)) data)
-         (gz i)).
+         (gz i)⎤.
 Proof.
   intros. subst t.
-  match goal with |- ?A |-- _ =>
-    erewrite (add_andp A (local (tc_environ Delta)))
-  end.
- 2: solve [apply andp_left1; unfold local, lift1; intro rho; apply prop_derives; intros [? ?]; auto].
-  match goal with |- ?A |-- _ =>
-    erewrite (add_andp A (local (`isptr (eval_var i (tarray (Tint sz sign noattr) n)))))
-  end.
-  2:{
-    go_lowerx. apply prop_right. eapply eval_var_isptr; eauto.
-    right; split; auto. rewrite <- H1; auto.
-   }
-  eapply derives_trans.
-  apply andp_right.
-  apply andp_left1. apply andp_left1. apply andp_left1. apply derives_refl.
-  apply andp_derives; [ apply andp_derives;
-    [ eapply unpack_globvar_star; try eassumption; try reflexivity
-    | apply derives_refl]  | apply derives_refl].
+  iIntros "(#? & H)".
+  iPoseProof (unpack_globvar_star with "[$H]") as "H"; first auto.
   rewrite H5.
-  rewrite <- andp_assoc.
-  apply andp_left1.
-  go_lowerx. 
-  eapply derives_trans; [| apply (id2pred_star_ZnthV_Tint Delta (globals_of_env rho)); auto].
-  instantiate (1 := rho).
- 2: rewrite <- H5; auto.
- match goal with |- ?F _ _ _ _ _ _ |-- _ => change F with @id2pred_star end.
-  subst gz.
-  normalize. clear H8.
-  rewrite H1 in H6.
+  rewrite -(id2pred_star_ZnthV_Tint Delta gz); auto.
+  iStopProof; go_lowerx.
+  rewrite monPred_at_intuitionistically.
+  fold id2pred_star.
+  iIntros "((% & ->) & $)"; iPureIntro.
   assert (headptr (globals_of_env rho i)). {
-    unfold globals_of_env. destruct  (globvar_eval_var _ _ _ _ H3 H H0) as [b [_ H10]]. rewrite H10.
-    exists b; auto. 
+    unfold globals_of_env. eapply globvar_eval_var in H0 as [b [_ H10]]; eauto. rewrite H10.
+    exists b; auto.
   }
   assert (align_compatible (Tint sz sign noattr) (globals_of_env rho i)). {
     destruct H7 as [b ?]. rewrite H7.
@@ -562,28 +503,30 @@ Proof.
     apply Z.divide_0_r.
   }
  apply headptr_isptr in H7.
- simpl andp. fold (sizeof (Tint sz sign noattr)).
-  assert (offset_strict_in_range (sizeof (Tint sz sign noattr) * n) (globals_of_env rho i)). {
-    unfold offset_strict_in_range.
-    destruct (globals_of_env rho i) eqn:?H; auto.
-    rewrite H5 in H6; simpl in H6. unfold sizeof in H6; simpl in H6.
-    pose proof initial_world.zlength_nonneg _ (gvar_init gv).
-    rewrite Z.max_r in H6 by lia.
-   change (match sz with I16 => 2 | I32 => 4 | _ => 1 end)
-    with (sizeof (Tint sz sign noattr)) in H6.
-    unfold Ptrofs.max_unsigned in H6.
-    pose proof init_data_list_size_pos (gvar_init gv).
-    simpl in H8.
-    unfold globals_of_env in H9. destruct (Map.get (ge_of rho) i) eqn:?H; inv H9.
-    rewrite Ptrofs.unsigned_zero.
-    split; try lia. 
-    rewrite Z.add_0_l.
-    apply Z.mul_nonneg_nonneg.
-    clear; pose proof (sizeof_pos (Tint sz sign noattr)); lia.
-    apply Zlength_nonneg.
-  }
-  normalize.
-  apply derives_refl.
+ split; first done; split; first done; split; last done.
+ unfold offset_strict_in_range.
+ destruct (globals_of_env rho i) eqn:?H; auto.
+ rewrite H1 H5 /= /sizeof /= in H6.
+ pose proof initial_world.zlength_nonneg _ (gvar_init gv).
+ rewrite -> Z.max_r in H6 by lia.
+ change (match sz with I16 => 2 | I32 => 4 | _ => 1 end)
+   with (sizeof (Tint sz sign noattr)) in H6.
+ unfold Ptrofs.max_unsigned in H6.
+ pose proof init_data_list_size_pos (gvar_init gv).
+ simpl in H8.
+ unfold globals_of_env in H9. destruct (Map.get (ge_of rho) i) eqn:?H; inv H9.
+ rewrite Ptrofs.unsigned_zero.
+ change (match sz with
+         | I16 => 2
+         | I32 => 4
+         | _ => 1
+         end) with (sizeof (Tint sz sign noattr)).
+ split; try lia.
+ rewrite Z.add_0_l.
+ apply Z.mul_nonneg_nonneg.
+ clear; pose proof (sizeof_pos (Tint sz sign noattr)); lia.
+   apply Zlength_nonneg.
+{ rewrite -H5 //. }
 Qed.
 
 Definition float_type (sz: floatsize) : Type :=
@@ -599,16 +542,16 @@ Lemma id2pred_star_ZnthV_tfloat  {cs: compspecs}:
  forall Delta sz gz sh n (v: val) (data: list (float_type sz)) mdata,
   n = Zlength mdata ->
   mdata = map (floattype2init_data sz) data ->
-  !! isptr v && !! align_compatible (Tfloat sz noattr) v &&
-  !! offset_strict_in_range (sizeof (Tfloat sz noattr) * n) v &&
-  `(id2pred_star Delta gz sh v mdata) |--
-  `(data_at sh (tarray (Tfloat sz noattr) n) (map  (float_constructor sz) data) v).
+  ⌜isptr v⌝ ∧ ⌜align_compatible (Tfloat sz noattr) v⌝ ∧
+  ⌜offset_strict_in_range (sizeof (Tfloat sz noattr) * n) v⌝ ∧
+  (⎡id2pred_star Delta gz sh v mdata⎤ : assert) ⊢
+  ⎡data_at sh (tarray (Tfloat sz noattr) n) (map  (float_constructor sz) data) v⎤.
 Proof. intros.
   subst n mdata.
   replace (Zlength (map  (floattype2init_data sz) data)) with (Zlength data)
     by (repeat rewrite Zlength_correct; rewrite map_length; auto).
   go_lowerx.
-  match goal with |- ?F _ _ _ _ _ _ |-- _ => change F with @id2pred_star end.
+  fold id2pred_star.
   change (offset_strict_in_range (sizeof (Tfloat sz noattr) * Zlength data) v) in H1.
   assert (offset_strict_in_range (sizeof (Tfloat sz noattr) * 0) v) by
     (unfold offset_strict_in_range; destruct v; auto; pose proof Ptrofs.unsigned_range i; lia).
@@ -621,7 +564,7 @@ revert v H H0 H1 H2; induction data; intros.
    unfold nested_field_type; simpl.
    rewrite data_at_rec_eq. unfold  aggregate_pred.aggregate_pred.array_pred.
   unfold aggregate_pred.array_pred. simpl.
-  repeat apply andp_right; auto; try apply prop_right; try reflexivity.  
+  repeat apply bi.and_intro; auto; try apply bi.pure_intro; try reflexivity.  
   hnf. simpl.
   split3; auto.
   split3; auto.
@@ -637,11 +580,11 @@ erewrite (split2_data_at_Tarray sh t (Z.succ (Zlength data)) 1).
 4: apply eq_refl.
 2: list_solve.
 2: list_solve. 2: auto. 2: list_solve. 2: apply eq_refl. 2: apply eq_refl.
-rewrite (sublist_one) by list_solve.
+rewrite -> (sublist_one) by list_solve.
 autorewrite with sublist.
 rewrite sublist_1_cons.
-rewrite sublist_same by list_solve.
-apply sepcon_derives.
+rewrite -> sublist_same by list_solve.
+apply bi.sep_mono.
 +
 clear IHdata.
 fold (tarray t 1). erewrite data_at_singleton_array_eq by apply eq_refl.
@@ -680,14 +623,14 @@ destruct sz; apply derives_refl.
    destruct v; try contradiction.
    pose proof (Ptrofs.unsigned_range i).
    assert (Ptrofs.max_unsigned = Ptrofs.modulus-1) by computable.
-   rewrite Z.mul_0_r in *.
+   rewrite -> Z.mul_0_r in *.
    assert (0 <= sizeof t * Zlength data) by (apply Z.mul_nonneg_nonneg; lia).
    unfold offset_strict_in_range, offset_val in *.
    unfold align_compatible in H0|-*.
    unfold Ptrofs.add.
-   rewrite (Ptrofs.unsigned_repr (sizeof t)) 
+   rewrite -> (Ptrofs.unsigned_repr (sizeof t))
     by (unfold sizeof, Ptrofs.max_unsigned, Ptrofs.modulus, Ptrofs.wordsize, Wordsize_Ptrofs.wordsize;
-          clear; subst t; destruct sz, Archi.ptr64; simpl; lia).
+          clear; subst t; destruct sz, Archi.ptr64; simpl; computable).
   rewrite Ptrofs.unsigned_repr.
   split3; try lia.
    assert (exists ch, access_mode t = By_value ch)
@@ -702,12 +645,12 @@ destruct sz; apply derives_refl.
   lia.
  }
  destruct H8 as [H8a [H8b H8c]].
-  eapply derives_trans; [ apply IHdata | ]; clear IHdata; auto.
+  etrans; [ apply IHdata | ]; clear IHdata; auto.
   replace (Z.succ (Zlength data) - 1) with (Zlength data) by (clear; lia).
-   apply derives_refl'; f_equal.
+   apply bi.equiv_entails_1_1; f_equal.
  unfold field_address0.
   rewrite if_true.
-  unfold offset_val. destruct v; simpl; auto. f_equal.
+  unfold offset_val. destruct v; simpl; auto. f_equiv; hnf.
   subst t; destruct sz; reflexivity.
   eapply field_compatible0_cons_Tarray.
   reflexivity.
@@ -716,7 +659,7 @@ destruct sz; apply derives_refl.
   split3; auto; red.
   unfold sizeof, Ctypes.sizeof;  fold Ctypes.sizeof. fold (sizeof t).
   pose proof (Zlength_nonneg data).
-  rewrite Z.max_r by lia.
+  rewrite -> Z.max_r by lia.
   unfold offset_strict_in_range in H1. rewrite Zlength_cons in H1.
   lia.
   apply align_compatible_rec_Tarray; intros.
@@ -737,49 +680,29 @@ Qed.
 
 Lemma unpack_globvar_array_float  {cs: compspecs}:
   forall t sz (data: list (float_type sz))  n Delta gz i gv,
-   (var_types Delta) ! i = None ->
-   (glob_types Delta) ! i = Some (gvar_info gv) ->
+   (var_types Delta) !! i = None ->
+   (glob_types Delta) !! i = Some (gvar_info gv) ->
    gvar_info gv = tarray t n ->
    gvar_volatile gv = false ->
    t = Tfloat sz noattr ->
    n = Zlength (gvar_init gv) ->
    gvar_init gv = map (floattype2init_data sz) data ->
    init_data_list_size (gvar_init gv) <= sizeof (gvar_info gv) <= Ptrofs.max_unsigned ->
-   local (`and (tc_environ Delta) (fun rho =>gz = globals_of_env rho)) && `(globvar2pred gz(i, gv)) |--
-      `(data_at (readonly2share (gvar_readonly gv))
+   local (`and (tc_environ Delta) (fun rho =>gz = globals_of_env rho)) ∧ ⎡globvar2pred gz(i, gv)⎤ ⊢
+      ⎡data_at (readonly2share (gvar_readonly gv))
          (tarray (Tfloat sz noattr) n)
          (map (float_constructor sz) data)
-         (gz i)).
+         (gz i)⎤.
 Proof.
   intros. subst t.
-  match goal with |- ?A |-- _ =>
-    erewrite (add_andp A (local (tc_environ Delta)))
-  end.
- 2: solve [apply andp_left1; unfold local, lift1; intro rho; apply prop_derives; intros [? ?]; auto].
-  match goal with |- ?A |-- _ =>
-    erewrite (add_andp A (local (`isptr (eval_var i (tarray (Tfloat sz noattr) n)))))
-  end.
-  2:{
-    go_lowerx. apply prop_right. eapply eval_var_isptr; eauto.
-    right; split; auto. rewrite <- H1; auto.
-   }
-  eapply derives_trans.
-  apply andp_right.
-  apply andp_left1. apply andp_left1. apply andp_left1. apply derives_refl.
-  apply andp_derives; [ apply andp_derives;
-    [ eapply unpack_globvar_star; try eassumption; try reflexivity
-    | apply derives_refl]  | apply derives_refl].
+  iIntros "(#? & H)".
+  iPoseProof (unpack_globvar_star with "[$H]") as "H"; first auto.
   rewrite H5.
-  rewrite <- andp_assoc.
-  apply andp_left1.
-  go_lowerx. 
-  eapply derives_trans; [| apply (id2pred_star_ZnthV_tfloat Delta sz (globals_of_env rho)); auto].
-  instantiate (1 := rho).
- 2: rewrite <- H5; auto.
- match goal with |- ?F _ _ _ _ _ _ |-- _ => change F with @id2pred_star end.
-  subst gz.
-  normalize. clear H8.
-  rewrite H1 in H6.
+  rewrite -(id2pred_star_ZnthV_tfloat Delta sz gz); auto.
+  iStopProof; go_lowerx.
+  rewrite monPred_at_intuitionistically.
+  fold id2pred_star.
+  iIntros "((% & ->) & $)"; iPureIntro.
   assert (headptr (globals_of_env rho i)). {
     unfold globals_of_env. destruct  (globvar_eval_var _ _ _ _ H3 H H0) as [b [_ H10]]. rewrite H10.
     exists b; auto. 
@@ -794,28 +717,25 @@ Proof.
     apply Z.divide_0_r.
   }
  apply headptr_isptr in H7.
- simpl andp. fold (sizeof (Tfloat sz noattr)).
-  assert (offset_strict_in_range (sizeof (Tfloat sz noattr) * n) (globals_of_env rho i)). {
-    unfold offset_strict_in_range.
-    destruct (globals_of_env rho i) eqn:?H; auto.
-    rewrite H5 in H6; simpl in H6. unfold sizeof in H6; simpl in H6.
-    pose proof initial_world.zlength_nonneg _ (gvar_init gv).
-    rewrite Z.max_r in H6 by lia.
-   change (match sz with F32 => 4 | F64 => 8 end)
-    with (sizeof (Tfloat sz noattr)) in H6.
-    unfold Ptrofs.max_unsigned in H6.
-    pose proof init_data_list_size_pos (gvar_init gv).
-    simpl in H8.
-    unfold globals_of_env in H9. destruct (Map.get (ge_of rho) i) eqn:?H; inv H9.
-    rewrite Ptrofs.unsigned_zero.
-    split; try lia. 
-    rewrite Z.add_0_l.
-    apply Z.mul_nonneg_nonneg.
-    clear; pose proof (sizeof_pos (Tfloat sz noattr)); lia.
-    apply Zlength_nonneg.
-  }
-  normalize.
-  apply derives_refl.
+ split; first done; split; first done; split; last done.
+ unfold offset_strict_in_range.
+ destruct (globals_of_env rho i) eqn:?H; auto.
+ rewrite H1 H5 /= /sizeof /= in H6.
+ pose proof initial_world.zlength_nonneg _ (gvar_init gv).
+ rewrite -> Z.max_r in H6 by lia.
+ change (match sz with F32 => 4 | F64 => 8 end)
+   with (sizeof (Tfloat sz noattr)) in *.
+ unfold Ptrofs.max_unsigned in H6.
+ pose proof init_data_list_size_pos (gvar_init gv).
+ simpl in H8.
+ unfold globals_of_env in H9. destruct (Map.get (ge_of rho) i) eqn:?H; inv H9.
+ rewrite Ptrofs.unsigned_zero.
+ split; try lia.
+ rewrite Z.add_0_l.
+ apply Z.mul_nonneg_nonneg.
+ clear; pose proof (sizeof_pos (Tfloat sz noattr)); lia.
+   apply Zlength_nonneg.
+{ rewrite -H5 //. }
 Qed.
 
 Definition gv_globvars2pred (gv: ident->val) (vl: list (ident * globvar type)) : mpred :=
@@ -850,84 +770,60 @@ Qed.
 
 Definition globvars_in_process (gv: globals) (done: list mpred)
                (halfdone: mpred)
-               (al: list (ident * globvar type)) (rho: environ) : mpred :=
- !! (gvars_denote gv rho) &&
- (fold_right_sepcon done * halfdone * globvars2pred gv al).
+               (al: list (ident * globvar type)) : assert :=
+ local (gvars_denote gv) ∧
+ ⎡fold_right_sepcon done ∗ halfdone ∗ globvars2pred gv al⎤.
+
+Context {Espec: OracleKind} `{!externalGS OK_ty Σ} {cs: compspecs}.
 
 Lemma start_globvars_in_process:
-  forall {cs: compspecs} {Espec: OracleKind} Delta P Q R
+  forall E Delta P Q R
           gz al SF c Post,
-  semax Delta
-    (PROPx P (LOCALx (gvars gz :: Q) (SEPx R)) *
-          globvars_in_process gz nil emp al * SF) c Post ->
-  semax Delta
-    (PROPx P (LOCALx (gvars gz :: Q) (SEPx R)) *
-     `(globvars2pred gz al) * SF) c Post.
+  semax E Delta
+    (PROPx P (LOCALx (gvars gz :: Q) (SEPx R)) ∗
+          globvars_in_process gz nil emp al ∗ SF) c Post ->
+  semax E Delta
+    (PROPx P (LOCALx (gvars gz :: Q) (SEPx R)) ∗
+     ⎡globvars2pred gz al⎤ ∗ SF) c Post.
 Proof.
 intros.
 eapply semax_pre; [ | apply H].
-apply andp_left2.
-intro rho.
-unfold PROPx, LOCALx, SEPx, local, lift1.
-unfold_lift.
-simpl. normalize.
-apply sepcon_derives; auto.
-apply sepcon_derives; auto.
-unfold globvars_in_process.
-rewrite prop_true_andp by auto.
-simpl.
-rewrite !emp_sepcon.
-unfold globvars2pred.
-auto.
+rewrite /globvars_in_process; go_lowerx.
+iIntros "(($ & (% & %) & $) & ? & $)"; auto.
 Qed.
 
 Lemma semax_process_globvars:
-  forall {cs: compspecs} {Espec: OracleKind} Delta P Q R R'
+  forall E Delta P Q R R'
           gz al SF c Post,
-  ENTAIL Delta, globvars_in_process gz R emp al |-- globvars_in_process gz R' emp nil ->
-  semax Delta
-    (PROPx P (LOCALx (gvars gz :: Q) (SEPx R')) * emp * SF) c Post ->
-  semax Delta
-    (PROPx P (LOCALx (gvars gz :: Q) (SEPx R)) *
-          `(globvars2pred gz al) * SF) c Post.
+  ENTAIL Delta, globvars_in_process gz R emp al ⊢ globvars_in_process gz R' emp nil ->
+  semax E Delta
+    (PROPx P (LOCALx (gvars gz :: Q) (SEPx R')) ∗ emp ∗ SF) c Post ->
+  semax E Delta
+    (PROPx P (LOCALx (gvars gz :: Q) (SEPx R)) ∗
+          ⎡globvars2pred gz al⎤ ∗ SF) c Post.
 Proof.
 intros.
 apply start_globvars_in_process.
 eapply semax_pre; [ | apply H0].
-intro rho.
-specialize (H rho).
-unfold PROPx, LOCALx, SEPx, local, lift1.
-simpl; normalize.
-unfold local, lift1 in H.
-simpl in H.
-rewrite prop_true_andp in H by auto.
-apply sepcon_derives; auto.
-clear - H.
-unfold globvars_in_process in *.
-simpl in *.
-normalize.
-rewrite !prop_true_andp in H by auto.
-match goal with |- _ * ?A |-- _ =>
- change A with (globvars2pred gz al)
-end.
-rewrite !sepcon_emp in H.
-eapply derives_trans; [ apply H | ].
-unfold globvars2pred, lift2; simpl; normalize.
+iIntros "(#? & ($ & $ & HR) & Hglob & $)".
+rewrite /globvars_in_process in H |- *.
+iPoseProof (H with "[-]") as "(_ & $ & _)".
+iDestruct "Hglob" as "($ & _ & $ & $)"; auto.
 Qed.
 
 Lemma process_globvar':
   forall {cs: compspecs} Delta done (i: ident)
           gz gv al (idata : init_data) t,
-       (var_types Delta) ! i = None ->
-       (glob_types Delta) ! i = Some t ->
+       (var_types Delta) !! i = None ->
+       (glob_types Delta) !! i = Some t ->
   (complete_legal_cosu_type (gvar_info gv) && is_aligned cenv_cs ha_env_cs la_env_cs (gvar_info gv) 0)%bool = true ->
        gvar_volatile gv = false ->
        gvar_info gv = t ->
        gvar_init gv = (idata::nil) ->
        init_data_size idata <= sizeof t ->
        sizeof t <= Ptrofs.max_unsigned ->
-  ENTAIL Delta,   
-       globvars_in_process gz done emp ((i,gv)::al) |--
+  ENTAIL Delta,
+       globvars_in_process gz done emp ((i,gv)::al) ⊢
     globvars_in_process gz done
             (id2pred_star Delta gz
                          (readonly2share (gvar_readonly gv))
@@ -939,21 +835,16 @@ pose proof  (unpack_globvar Delta gz i t gv idata H H0 H1 H2 H3 H4 H5 H6).
 clear H H0 H1 H2 H3 H4 H5 H6.
 unfold globvars_in_process.
 unfold globvars2pred.
-change (lift_S (LiftEnviron Prop)) with environ in *.
-go_lowerx. unfold lift2.
-normalize.
-rewrite sepcon_assoc.
-apply sepcon_derives; auto.
-apply sepcon_derives; auto.
-unfold local, lift1 in H7. specialize (H7 rho). simpl in H7. rewrite prop_true_andp in H7 by (split; auto).
-apply H7.
+go_lowerx.
+iIntros "($ & $ & ? & $)".
+iApply (H7 with "[-]"); iFrame; eauto.
 Qed.
 
 Lemma process_globvar_array:
-  forall {cs: compspecs} Delta done gz (i: ident)
+  forall Delta done gz (i: ident)
           gv al (n: Z) (t: type)  (sz : intsize) (sign : signedness) (data : list int),
-       (var_types Delta) ! i = None ->
-       (glob_types Delta) ! i = Some (gvar_info gv) ->
+       (var_types Delta) !! i = None ->
+       (glob_types Delta) !! i = Some (gvar_info gv) ->
        gvar_info gv = tarray t n ->
        gvar_volatile gv = false ->
        t = Tint sz sign noattr ->
@@ -963,12 +854,12 @@ Lemma process_globvar_array:
        init_data_list_size (gvar_init gv) <= sizeof (gvar_info gv) <=
        Ptrofs.max_unsigned ->
   ENTAIL Delta,   
-       globvars_in_process gz done emp ((i,gv)::al) |--
+       globvars_in_process gz done emp ((i,gv)::al) ⊢
     globvars_in_process gz 
         (data_at
                    (readonly2share (gvar_readonly gv))
                    (tarray (Tint sz sign noattr) n)
-                   (map (Vint oo Cop.cast_int_int sz sign) data) (gz i) :: done)
+                   (map (Basics.compose Vint (Cop.cast_int_int sz sign)) data) (gz i) :: done)
         emp al.
 Proof.
 intros.
@@ -976,21 +867,13 @@ pose proof (unpack_globvar_array _ _ _ _ _ _ gz _ _ H H0 H1 H2 H3 H4 H5 H6 H7).
 clear H H0 H1 H2 H3 H4 H5 H6 H7.
 unfold globvars_in_process.
 unfold globvars2pred.
-change (lift_S (LiftEnviron Prop)) with environ in *.
-unfold lift2.
-change  (fun rho : environ => gz = globals_of_env rho)
-  with (locald_denote (gvars gz)) in H8|-*.
 go_lowerx.
-normalize.
-pull_right (fold_right_sepcon done).
-apply sepcon_derives; auto.
-apply sepcon_derives; auto.
-unfold local, lift1 in H8. specialize (H8 rho). simpl in H8. rewrite prop_true_andp in H8 by (split; auto).
-apply H8.
+iIntros "($ & $ & ? & $)".
+iApply (H8 with "[-]"); iFrame; eauto.
 Qed.
 
 Lemma process_globvar_array_float:
-  forall {cs: compspecs} Delta done gz (i: ident)
+  forall Delta done gz (i: ident)
           gv al (n: Z) (t: type)  (sz : floatsize)
          (data : list (float_type sz)),
        Maps.PTree.get i (var_types Delta) = None ->
@@ -1002,8 +885,8 @@ Lemma process_globvar_array_float:
        gvar_init gv = map (floattype2init_data sz) data ->
        init_data_list_size (gvar_init gv) <= sizeof (gvar_info gv) <=
        Ptrofs.max_unsigned ->
-  ENTAIL Delta,   
-       globvars_in_process gz done emp ((i,gv)::al) |--
+  ENTAIL Delta,
+       globvars_in_process gz done emp ((i,gv)::al) ⊢
     globvars_in_process gz 
         (data_at
                    (readonly2share (gvar_readonly gv))
@@ -1016,27 +899,19 @@ assert (H8 := unpack_globvar_array_float _ _ _ _ _ gz _ _ H H0 H1 H2 H3 H4 H5 H6
 clear H H0 H1 H2 H3 H4 H5 H6.
 unfold globvars_in_process.
 unfold globvars2pred.
-change (lift_S (LiftEnviron Prop)) with environ in *.
-unfold lift2.
-change  (fun rho : environ => gz = globals_of_env rho)
-  with (locald_denote (gvars gz)) in H8|-*.
 go_lowerx.
-normalize.
-pull_right (fold_right_sepcon done).
-apply sepcon_derives; auto.
-apply sepcon_derives; auto.
-unfold local, lift1 in H8. specialize (H8 rho). simpl in H8. rewrite prop_true_andp in H8 by (split; auto).
-apply H8.
+iIntros "($ & $ & ? & $)".
+iApply (H8 with "[-]"); iFrame; eauto.
 Qed.
 
 Lemma process_globvar_star':
   forall {cs: compspecs} Delta done gz (i: ident)
           gv al,
-       (var_types Delta) ! i = None ->
-       (glob_types Delta) ! i = Some (gvar_info gv) ->
+       (var_types Delta) !! i = None ->
+       (glob_types Delta) !! i = Some (gvar_info gv) ->
        gvar_volatile gv = false ->
-  ENTAIL Delta,   
-       globvars_in_process gz done emp ((i,gv)::al) |--
+  ENTAIL Delta,
+       globvars_in_process gz done emp ((i,gv)::al) ⊢
     globvars_in_process gz done
             (id2pred_star Delta gz
                          (readonly2share (gvar_readonly gv))
@@ -1047,39 +922,30 @@ intros.
 assert (H5 := unpack_globvar_star _ gz _ _ H H0 H1).
 clear H H0 H1.
 unfold globvars_in_process, globvars2pred.
-change (lift_S (LiftEnviron Prop)) with environ in *.
-unfold lift2.
-change  (fun rho : environ => gz = globals_of_env rho)
-  with (locald_denote (gvars gz)) in H5|-*.
 go_lowerx.
-normalize.
-rewrite sepcon_assoc.
-apply sepcon_derives; auto.
-apply sepcon_derives; auto.
-unfold local, lift1 in H5. specialize (H5 rho). simpl in H5.
-rewrite prop_true_andp in H5 by (split; auto).
-apply H5.
+iIntros "($ & _ & ? & $)".
+iApply (H5 with "[-]"); iFrame; eauto.
 Qed.
 
 Fixpoint init_datalist2pred' {cs: compspecs}
      (Delta: tycontext) (gv: globals) (dl: list init_data)  (sh: share) (ofs: Z) (v: val) : mpred :=
  match dl with
  | d::dl' => init_data2pred' Delta gv d sh (offset_val ofs v) 
-                * init_datalist2pred' Delta gv dl' sh (ofs + init_data_size d) v
+                ∗ init_datalist2pred' Delta gv dl' sh (ofs + init_data_size d) v
  | nil => emp
  end.
 
 Lemma halfprocess_globvar_star:
   forall {cs: compspecs} Delta done gz (i: ident)
           gv al,
-       (var_types Delta) ! i = None ->
-       (glob_types Delta) ! i = Some (gvar_info gv) ->
+       (var_types Delta) !! i = None ->
+       (glob_types Delta) !! i = Some (gvar_info gv) ->
   (complete_legal_cosu_type (gvar_info gv) && is_aligned cenv_cs ha_env_cs la_env_cs (gvar_info gv) 0)%bool = true ->
        gvar_volatile gv = false ->
        init_data_list_size (gvar_init gv) <= sizeof (gvar_info gv) <=
        Ptrofs.max_unsigned ->
   ENTAIL Delta,   
-       globvars_in_process gz done emp ((i,gv)::al) |--
+       globvars_in_process gz done emp ((i,gv)::al) ⊢
     globvars_in_process gz
        (init_datalist2pred' Delta gz (gvar_init gv) (readonly2share (gvar_readonly gv)) 0 (gz i) :: done)
             emp  al.
@@ -1088,11 +954,7 @@ intros.
 unfold globvars_in_process.
 unfold globvars2pred; fold globvars2pred.
 go_lowerx.
-unfold lift2. simpl.
-normalize.
-pull_right (fold_right_sepcon done).
-apply sepcon_derives; auto.
-cancel.
+iIntros "($ & _ & H & $)".
 unfold globvar2pred.
 simpl.
 rewrite H2.
@@ -1102,22 +964,19 @@ replace gz with (globals_of_env rho).
 rewrite <- offset_zero_globals_of_env at 1.
 set (ofs:=0).
 clearbody ofs.
-revert ofs; induction (gvar_init gv); intros.
-apply derives_refl.
-apply sepcon_derives.
-destruct (globvar_eval_var _ _ _ _ H4 H H0) as [b [? ?]].
-eapply init_data2pred_rejigger; eauto.
-unfold globals_of_env.
-rewrite H8. reflexivity.
-fold init_data_list2pred.
-fold init_datalist2pred'.
-spec IHl.
-simpl in H3.
-pose proof (init_data_size_pos a).
-lia.
-eapply derives_trans; [ | apply IHl].
-rewrite offset_offset_val.
-auto.
+iInduction (gvar_init gv)as [|] "IH" forall (ofs); simpl.
+{ done. }
+iDestruct "H" as "(H & ?)"; iSplitL "H".
+- destruct (globvar_eval_var _ _ _ _ H4 H H0) as [b [? ?]].
+  iApply init_data2pred_rejigger; eauto.
+  unfold globals_of_env.
+  rewrite H8. reflexivity.
+- iApply "IH".
+  + iPureIntro.
+    simpl in H3.
+    pose proof (init_data_size_pos a).
+    lia.
+  + rewrite offset_offset_val //.
 Qed.
 
 Lemma map_instantiate:
@@ -1140,33 +999,26 @@ normalize. destruct rho; simpl.
 unfold gvars_denote. unfold_lift. unfold local, lift1.
 rewrite sepcon_comm. unfold Clight_seplog.mkEnv; simpl. unfold seplog.globals_only, globals_of_env; simpl.
 apply pred_ext; normalize.
-+ apply andp_right. apply prop_right. intuition. trivial.
-+ apply andp_right. apply prop_right. intuition. trivial.
++ apply bi.and_intro. apply bi.pure_intro. intuition. trivial.
++ apply bi.and_intro. apply bi.pure_intro. intuition. trivial.
 Qed.
  *)
 
-Definition main_pre_old {Z: Type} (prog: Clight.program) (ora: Z) : globals -> environ -> mpred :=
-fun gv rho => 
-  !! (gv = globals_of_env rho) &&
-   (globvars2pred gv (prog_vars prog) * has_ext ora).
+Definition main_pre_old (prog: Clight.program) (ora: OK_ty) (gv: globals) : assert :=
+local (fun rho => gv = globals_of_env rho) ∧
+   ⎡globvars2pred gv (prog_vars prog) ∗ has_ext ora⎤.
 
 Lemma main_pre_start_old:
- forall {Z} prog gv (ora : Z),
-   main_pre_old prog ora gv = (PROP() LOCAL(gvars gv) SEP(has_ext ora))%assert * `(globvars2pred gv (prog_vars prog)).
+ forall prog gv ora,
+   main_pre_old prog ora gv ⊣⊢ (PROP() LOCAL(gvars gv) SEP(has_ext ora))%assert ∗ ⎡globvars2pred gv (prog_vars prog)⎤.
 Proof.
 intros.
 unfold main_pre_old.
 unfold globvars2pred,  PROPx, LOCALx, SEPx.
-unfold lift2.
-extensionality rho.
-simpl.
+split => rho; monPred.unseal.
+unfold_lift; rewrite /lift1.
 normalize.
-unfold gvars_denote. unfold_lift. unfold local, lift1.
-fold (globals_of_env rho).
-rewrite sepcon_comm.
-apply pred_ext; intros; normalize.
-rewrite prop_true_andp by auto.
-auto.
+rewrite and_True True_and bi.sep_comm //.
 Qed.
 
 (*
@@ -1190,12 +1042,12 @@ apply (initdata_list2pred_ge_eq RS).
 Qed.
 
 Lemma globvars2pred_ge_eq_entails {rho sigma gz} (RS: ge_of rho = ge_of sigma):
-      forall l, globvars2pred gz l rho |-- globvars2pred gz l sigma.
+      forall l, globvars2pred gz l rho ⊢ globvars2pred gz l sigma.
 Proof.
 unfold globvars2pred, lift2. induction l.
 + simpl. unfold globals_of_env; rewrite RS; trivial.
 + eapply derives_trans. simpl. rewrite sepcon_comm, <- sepcon_andp_prop'.
-  apply sepcon_derives. apply IHl. apply derives_refl. clear IHl.
+  apply bi.sep_mono. apply IHl. apply derives_refl. clear IHl.
   simpl. rewrite sepcon_andp_prop', sepcon_comm, (globvar2pred_ge_eq RS). trivial.
 Qed.
 
@@ -1204,18 +1056,14 @@ Lemma globvars2pred_ge_eq {rho sigma gz l} (RS: ge_of rho = ge_of sigma):
 Proof. apply pred_ext; apply globvars2pred_ge_eq_entails; [ | symmetry]; trivial. Qed.
  *)
 
-Lemma close_precondition_main {Z p ora gv}:
-close_precondition nil (@main_pre Z p ora gv) = @main_pre_old Z p ora gv.
+Lemma close_precondition_main {p ora gv}:
+close_precondition nil (main_pre p ora gv) ⊣⊢ main_pre_old p ora gv.
 Proof.
-unfold close_precondition; extensionality rho.
-unfold main_pre, main_pre_old; simpl snd. 
-forget (prog_vars p) as vars. clear p.
-remember (globvars2pred gv vars) as G.
-apply pred_ext.
-+ apply exp_left. intros vals. normalize.
-+ Exists (@nil val). 
-  apply andp_right. apply prop_right; split; [trivial | constructor].
-  clear HeqG. normalize. rewrite prop_true_andp; auto.
+rewrite /close_precondition /main_pre /main_pre_old.
+split => rho; simpl; monPred.unseal; rewrite /lift1.
+iSplit.
+- iIntros "H"; iDestruct "H" as (? _ (-> & ?)) "$"; auto.
+- iIntros "(% & $)"; iExists []; auto.
 Qed.
 
 
@@ -1223,16 +1071,16 @@ Lemma process_globvar_space0:
   forall {cs: compspecs} Delta done (i: ident)
           gz gv al t,
        gvar_info gv = t ->
-       (var_types Delta) ! i = None ->
-       (glob_types Delta) ! i = Some t ->
+       (var_types Delta) !! i = None ->
+       (glob_types Delta) !! i = Some t ->
   (complete_legal_cosu_type (gvar_info gv)
    && is_aligned cenv_cs ha_env_cs la_env_cs (gvar_info gv) 0
    && fully_nonvolatile (rank_type cenv_cs t) t)%bool = true ->
        gvar_volatile gv = false ->
        gvar_init gv = (Init_space (sizeof t)::nil) ->
        sizeof t <= Ptrofs.max_unsigned ->
-  ENTAIL Delta,   
-       globvars_in_process gz done emp ((i,gv)::al) |--
+  ENTAIL Delta,
+       globvars_in_process gz done emp ((i,gv)::al) ⊢
     globvars_in_process gz
        (data_at (readonly2share (gvar_readonly gv)) t  (zero_val t) (gz i) :: done)
             emp  al.
@@ -1241,44 +1089,35 @@ intros until t. intros H3; intros.
 rewrite andb_true_iff in H1. destruct H1 as [H1 Hvol].
 assert (H7 := unpack_globvar Delta gz i t gv _ H H0 H1 H2 H3 H4).
 spec H7.
-simpl. pose proof (sizeof_pos t). rewrite Z.max_l by lia. lia.
+simpl. pose proof (sizeof_pos t). rewrite -> Z.max_l by lia. lia.
 specialize (H7 H5).
-go_lowerx.
 unfold globvars_in_process.
 unfold globvars2pred; fold globvars2pred.
-unfold lift2. simpl. normalize.
-pull_right (fold_right_sepcon done).
-apply sepcon_derives; auto.
-apply sepcon_derives; auto.
-specialize (H7 rho).
-unfold_lift in H7. unfold local, lift1 in H7.
-simpl in H7.
-rewrite prop_true_andp in H7 by auto.
-eapply derives_trans; [ apply H7  | ].
-rewrite andb_true_iff in H1.
-destruct H1.
-rewrite H3 in *.
-apply mapsto_zero_data_at_zero; auto.
-apply readable_readonly2share.
-pose proof (la_env_cs_sound 0 t H1 H9).
-apply headptr_field_compatible; auto.
-eapply go_lower.gvars_denote_HP; eauto.
-red; auto.
-rep_lia.
+go_lowerx.
+iIntros "($ & $ & ? & $)".
+apply andb_true_iff in H1 as [H1 H9].
+rewrite -> H3 in *.
+iApply mapsto_zero_data_at_zero; last iApply H7; auto.
+- apply readable_readonly2share.
+- pose proof (la_env_cs_sound 0 t H1 H9).
+  apply headptr_field_compatible; auto.
+  + eapply go_lower.gvars_denote_HP; eauto.
+  + red; auto.
+  + rep_lia.
 Qed.
 
 Lemma process_globvar_space:
   forall {cs: compspecs} Delta done (i: ident)
           gz gv al t,
        gvar_info gv = t ->
-       (var_types Delta) ! i = None ->
-       (glob_types Delta) ! i = Some t ->
+       (var_types Delta) !! i = None ->
+       (glob_types Delta) !! i = Some t ->
   (complete_legal_cosu_type (gvar_info gv) && is_aligned cenv_cs ha_env_cs la_env_cs (gvar_info gv) 0)%bool = true ->
        gvar_volatile gv = false ->
        gvar_init gv = (Init_space (sizeof t)::nil) ->
        sizeof t <= Ptrofs.max_unsigned ->
-  ENTAIL Delta,   
-       globvars_in_process gz done emp ((i,gv)::al) |--
+  ENTAIL Delta,
+       globvars_in_process gz done emp ((i,gv)::al) ⊢
     globvars_in_process gz
        (data_at_  (readonly2share (gvar_readonly gv)) t (gz i) :: done)
             emp  al.
@@ -1286,48 +1125,37 @@ Proof.
 intros until t. intros H3; intros.
 assert (H7 := unpack_globvar Delta gz i t gv _ H H0 H1 H2 H3 H4).
 spec H7.
-simpl. pose proof (sizeof_pos t). rewrite Z.max_l by lia. lia.
+simpl. pose proof (sizeof_pos t). rewrite -> Z.max_l by lia. lia.
 specialize (H7 H5).
-go_lowerx.
 unfold globvars_in_process.
 unfold globvars2pred; fold globvars2pred.
-unfold lift2. simpl. normalize.
-pull_right (fold_right_sepcon done).
-apply sepcon_derives; auto.
-apply sepcon_derives; auto.
-specialize (H7 rho).
-unfold_lift in H7. unfold local, lift1 in H7.
-simpl in H7.
-rewrite prop_true_andp in H7 by auto.
-eapply derives_trans; [ apply H7  | ].
-eapply derives_trans. apply mapsto_zeros_memory_block.
-destruct (gvar_readonly gv); simpl; auto. apply readable_Ers.
-assert_PROP (isptr (gz i)) by (saturate_local; apply prop_right; auto).
-assert (headptr (gz i)).
-rewrite H8 in *. destruct (Map.get (ge_of rho) i); try contradiction. hnf; eauto.
-rewrite memory_block_data_at_; auto.
-subst t.
-rewrite andb_true_iff in H1; destruct H1.
-pose proof (la_env_cs_sound 0 (gvar_info gv) H1 H3).
-apply headptr_field_compatible; auto.
-apply I.
-assert (Ptrofs.modulus = Ptrofs.max_unsigned + 1) by computable.
-lia.
+go_lowerx.
+iIntros "($ & $ & ? & $)".
+apply andb_true_iff in H1 as [H1 H9].
+rewrite -> H3 in *.
+iApply memory_block_data_at_.
+{ subst t.
+  pose proof (la_env_cs_sound 0 (gvar_info gv) H1 H9).
+  apply headptr_field_compatible; auto.
+  + eapply go_lower.gvars_denote_HP; eauto.
+  + red; auto.
+  + rep_lia. }
+iApply mapsto_zeros_memory_block; iApply H7; auto.
 Qed.
 
 Lemma process_globvar_ptrarray_space:
-  forall {cs: compspecs} Delta done (i: ident)
+  forall Delta done (i: ident)
           gz gv al t t' n,
        t = Tarray (Tpointer t' noattr) n noattr ->
        gvar_info gv = t ->
-       (var_types Delta) ! i = None ->
-       (glob_types Delta) ! i = Some t ->
+       (var_types Delta) !! i = None ->
+       (glob_types Delta) !! i = Some t ->
   (complete_legal_cosu_type (gvar_info gv) && is_aligned cenv_cs ha_env_cs la_env_cs (gvar_info gv) 0)%bool = true ->
        gvar_volatile gv = false ->
        gvar_init gv = (Init_space (sizeof t)::nil) ->
        sizeof t <= Ptrofs.max_unsigned ->
   ENTAIL Delta,   
-       globvars_in_process gz done emp ((i,gv)::al) |--
+       globvars_in_process gz done emp ((i,gv)::al) ⊢
     globvars_in_process gz
        (data_at  (readonly2share (gvar_readonly gv)) (Tarray (Tpointer t' noattr) n noattr)
                                   (Zrepeat nullval n)  (gz i) :: done)
@@ -1336,76 +1164,63 @@ Proof.
 intros until n. intros Ht H3; intros.
 assert (H7 := unpack_globvar Delta gz i t gv _ H H0 H1 H2 H3 H4).
 spec H7.
-simpl. pose proof (sizeof_pos t). rewrite Z.max_l by lia. lia.
+simpl. pose proof (sizeof_pos t). rewrite -> Z.max_l by lia. lia.
 specialize (H7 H5).
-go_lowerx.
 unfold globvars_in_process.
 unfold globvars2pred; fold globvars2pred.
-unfold lift2.
-simpl.
-normalize.
-pull_right (fold_right_sepcon done).
-apply sepcon_derives; auto.
-apply sepcon_derives; auto.
-specialize (H7 rho).
-unfold_lift in H7. unfold local, lift1 in H7.
-simpl in H7.
-rewrite prop_true_andp in H7 by auto.
-eapply derives_trans; [ apply H7  | ].
+go_lowerx.
+iIntros "($ & $ & ? & $)".
+apply andb_true_iff in H1 as [H1 H9].
+rewrite -> H3 in *.
+iPoseProof (H7 with "[-]") as "H"; first auto; simpl.
 subst t; simpl.
 destruct (zlt n 0).
 -
 unfold sizeof; simpl.
-rewrite Z.max_l by lia.
-simpl.
+rewrite -> Z.max_l by lia.
 rewrite Z.mul_0_r.
 assert (readable_share (readonly2share (gvar_readonly gv)))
   by apply readable_readonly2share.
 forget  (readonly2share (gvar_readonly gv)) as sh.
 unfold mapsto_zeros.
-destruct (gz i); try apply FF_left.
-normalize.
+destruct (gz i); try done.
 unfold data_at, field_at.
 change (nested_field_offset _ _) with 0.
 unfold at_offset.
 unfold nested_field_type; simpl.
-normalize.
 rewrite data_at_rec_eq.
-rewrite Z.max_l by lia.
+rewrite -> Z.max_l by lia.
 change (unfold_reptype _) with (repeat nullval (Z.to_nat n)).
-rewrite Z2Nat_neg by auto.  simpl repeat.
-rewrite aggregate_pred.aggregate_pred.array_pred_len_0 by auto.
-change predicates_sl.emp with emp.
-apply andp_right; auto.
-apply prop_right.
+rewrite -> Z2Nat_neg by auto.  simpl repeat.
+rewrite -> aggregate_pred.aggregate_pred.array_pred_len_0 by auto.
+iDestruct "H" as "(% & _)"; iPureIntro.
+split; last done.
 split3; auto. apply I.
 split3.
 simpl. unfold sizeof; simpl.  lia.
 2: apply I.
-red. constructor; auto. intros. lia. 
+red. constructor; auto. intros. lia.
 -
-unfold sizeof; simpl.
-rewrite Z.max_r by lia.
+rewrite -> Z.max_r by lia.
 unfold data_at.
 erewrite @field_at_Tarray with (n:=n);
   [ | apply I | reflexivity | lia | apply JMeq_refl].
 unfold mapsto_zeros.
-destruct (gz i) eqn:?H;
- try apply FF_left.
-normalize.
+destruct (gz i) eqn:?H; try done.
+iDestruct "H" as "(% & H)".
 assert (field_compatible0 (Tarray (Tpointer t' noattr) n noattr) (ArraySubsc 0::nil) (gz i)).
-{ rewrite H9; split3; auto. apply I. split; auto. simpl. unfold sizeof; simpl.
-   rewrite Z.max_r by lia. lia.
+{ rewrite H10; split3; auto. apply I. split; auto. simpl. unfold sizeof; simpl.
+   rewrite -> Z.max_r by lia. lia.
   split. red. apply align_compatible_rec_Tarray. intros.
      eapply align_compatible_rec_by_value. reflexivity.
      simpl.
-  rewrite H8 in H9; unfold globals_of_env in H9. destruct (Map.get (ge_of rho) i); inv H9.
+  rewrite H8 in H10; unfold globals_of_env in H10. destruct (Map.get (ge_of rho) i); inv H10.
   normalize. apply Z.divide_mul_l. unfold Mptr.  destruct Archi.ptr64; exists 1; simpl; auto.
   simpl. split; auto. lia.
 }
 assert (Halign: (align_chunk Mptr | Ptrofs.unsigned i0)). {
-  rewrite H8 in H9;
- clear - H9. unfold globals_of_env in H9. destruct (Map.get (ge_of rho) i); inv H9.
+  rewrite H8 in H10;
+ clear - H10. unfold globals_of_env in H10. destruct (Map.get (ge_of rho) i); inv H10.
  apply Z.divide_0_r.
 }
 forget (gz i) as p.
@@ -1419,119 +1234,110 @@ rewrite prop_true_andp.
 destruct H12 as [? [? [? [? [? ?]]]]].
 split3; auto. split3; auto. simpl; split; auto. lia.
 }
-apply andp_right.
-apply prop_right. autorewrite with sublist. auto.
-rewrite Z2Nat.inj_mul; [ | destruct Archi.ptr64; lia| lia].
-rewrite Z2Nat.inj_sub by lia.
+iSplit.
+{ autorewrite with sublist; auto. }
+rewrite -> Z2Nat.inj_mul; [ | destruct Archi.ptr64; lia| lia].
+rewrite -> Z2Nat.inj_sub by lia.
 change (Z.to_nat 0) with O. rewrite Nat.sub_0_r.
 unfold nested_field_type; simpl.
 unfold nested_field_offset; simpl.
 unfold at_offset.
 rewrite <- (Z2Nat.id n) in H11 by lia.
 unfold Zrepeat.
-clear - H10 H11 H13 Halign.
-revert i0 H10 H11 Halign; induction (Z.to_nat n); intros; simpl.
-rewrite Nat.mul_0_r; apply derives_refl.
+clear - H11 H13 Halign.
+rewrite mapsto_memory_block.address_mapsto_zeros_eq.
+iInduction (Z.to_nat n) as [|] "IH" forall (i0 H11 Halign); intros; simpl.
+{ done. }
 autorewrite with sublist. normalize.
-rewrite mapsto_memory_block.address_mapsto_zeros_eq in *.
-rewrite Nat2Z.inj_mul.
-rewrite Z2Nat.id by (destruct Archi.ptr64; computable).
+rewrite !Nat2Z.inj_mul.
+rewrite -> Z2Nat.id by (destruct Archi.ptr64; computable).
 rewrite inj_S. unfold Z.succ.
 rewrite Z.add_comm.
-rewrite Z.mul_add_distr_l.
-rewrite Z.mul_1_r.
-rewrite mapsto_memory_block.address_mapsto_zeros'_split by (destruct Archi.ptr64; rep_lia).
-change (predicates_sl.sepcon ?A ?B) with (A*B).
-apply sepcon_derives.
-unfold data_at_rec;  simpl.
-unfold mapsto. simpl. rewrite if_true by apply H13.
-rewrite andb_false_r.
-apply orp_right1.
-rewrite prop_true_andp by apply mapsto_memory_block.is_pointer_or_null_nullval.
-{
-change (if Archi.ptr64 then 8 else 4) with (size_chunk Mptr). constructor.
-apply mapsto_memory_block.address_mapsto_address_mapsto_zeros; auto.
-}
-unfold adr_add.
-simpl.
-assert (H20: 0 <= (if Archi.ptr64 then 8 else 4) <= Ptrofs.max_unsigned)
-  by (destruct Archi.ptr64; clear; rep_lia).
-change (if Archi.ptr64 then 8 else 4) with (size_chunk Mptr) in *.
-specialize (IHn0 (Ptrofs.add i0 (Ptrofs.repr (size_chunk Mptr)))).
-rewrite Nat2Z.inj_mul in IHn0 by lia.
-rewrite Z2Nat.id in IHn0 by lia.
-replace (Ptrofs.unsigned i0 + (size_chunk Mptr))
+rewrite -> Z.mul_add_distr_l.
+rewrite -> Z.mul_1_r.
+rewrite -> mapsto_memory_block.address_mapsto_zeros'_split by (destruct Archi.ptr64; rep_lia).
+iDestruct "H" as "(H & ?)"; iSplitL "H".
++ unfold data_at_rec; simpl.
+  unfold mapsto. simpl. rewrite -> if_true by done.
+  rewrite andb_false_r.
+  iLeft.
+  rewrite -> prop_true_andp by apply mapsto_memory_block.is_pointer_or_null_nullval.
+  iApply mapsto_memory_block.address_mapsto_address_mapsto_zeros; auto.
++ unfold adr_add.
+  simpl.
+  assert (H20: 0 <= (if Archi.ptr64 then 8 else 4) <= Ptrofs.max_unsigned)
+    by (destruct Archi.ptr64; clear; rep_lia).
+  change (if Archi.ptr64 then 8 else 4) with (size_chunk Mptr) in *.
+  iSpecialize ("IH" $! (Ptrofs.add i0 (Ptrofs.repr (size_chunk Mptr)))).
+  replace (Ptrofs.unsigned i0 + (size_chunk Mptr))
   with (Ptrofs.unsigned
-           (Ptrofs.add i0 (Ptrofs.repr (size_chunk Mptr)))). 
-eapply derives_trans; [eapply IHn0 | ].
-rep_lia.
-rewrite inj_S in H11.
-unfold Ptrofs.add.
-rewrite Ptrofs.unsigned_repr.
-rewrite Ptrofs.unsigned_repr by lia.
-lia.
-rewrite Ptrofs.unsigned_repr by lia.
-rep_lia.
-clear - Halign H10 H11 H20.
-unfold Ptrofs.add. rewrite Ptrofs.unsigned_repr.
-apply Z.divide_add_r; auto.
-rewrite Ptrofs.unsigned_repr by lia.
-apply align_size_chunk_divides.
-rewrite Ptrofs.unsigned_repr by lia.
-rep_lia.
-apply aggregate_pred.rangespec_shift_derives.
-intros.
-rewrite Z.sub_0_r in H0. subst i.
-rewrite !Z.sub_0_r.
-rewrite Znth_pos_cons by lia.
-rewrite <- (Nat2Z.id n0).
-rewrite Znth_repeat_inrange by lia.
-apply derives_refl'. f_equal. 
-simpl.
-f_equal.
-rewrite Ptrofs.add_assoc. f_equal.
-rewrite ptrofs_add_repr.
-f_equal. simpl; unfold sizeof; simpl.
-  change (if Archi.ptr64 then 8 else 4) with (size_chunk Mptr). lia.
-unfold Ptrofs.add.
-rewrite Ptrofs.unsigned_repr.
-2:{
-rewrite Ptrofs.unsigned_repr by (destruct Archi.ptr64; rep_lia).
-destruct Archi.ptr64; rep_lia.
-}
-reflexivity.
+           (Ptrofs.add i0 (Ptrofs.repr (size_chunk Mptr)))).
+  iPoseProof ("IH" with "[%] [%] [$]") as "?".
+  { split; first rep_lia.
+    rewrite inj_S in H11.
+    unfold Ptrofs.add.
+    rewrite Ptrofs.unsigned_repr.
+    rewrite -> Ptrofs.unsigned_repr by lia.
+    lia.
+    rewrite -> Ptrofs.unsigned_repr by lia.
+    rep_lia. }
+  { unfold Ptrofs.add. rewrite Ptrofs.unsigned_repr.
+    apply Z.divide_add_r; auto.
+    rewrite -> Ptrofs.unsigned_repr by lia.
+    apply align_size_chunk_divides.
+    rewrite -> Ptrofs.unsigned_repr by lia.
+    rep_lia. }
+  iApply (aggregate_pred.rangespec_shift_derives with "[$]").
+  intros.
+  rewrite Z.sub_0_r in H0. subst i.
+  rewrite !Z.sub_0_r.
+  rewrite -> Znth_pos_cons by lia.
+  rewrite <- (Nat2Z.id n0).
+  rewrite -> !Znth_repeat_inrange by lia.
+  apply bi.equiv_entails_1_1. f_equiv; hnf; simpl.
+  rewrite Ptrofs.add_assoc. f_equal.
+  rewrite ptrofs_add_repr.
+  f_equal. f_equal. lia.
+  { unfold Ptrofs.add.
+    rewrite Ptrofs.unsigned_repr //.
+    rewrite -> Ptrofs.unsigned_repr by (destruct Archi.ptr64; rep_lia).
+    rep_lia. }
 Qed.
 
 Lemma process_globvar_extern:
  forall {CS: compspecs} Delta done gz i gv al,
        gvar_init gv = nil ->
        gvar_volatile gv = false ->
-  ENTAIL Delta,   
-       globvars_in_process gz done emp ((i,gv)::al) |--
+  ENTAIL Delta,
+       globvars_in_process gz done emp ((i,gv)::al) ⊢
     globvars_in_process gz done emp  al.
 Proof.
 intros.
-apply andp_left2.
 unfold globvars_in_process.
-intro rho.
-unfold globvars2pred, lift2.
-apply andp_derives; auto.
-simpl.
-normalize.
-apply sepcon_derives; auto.
-unfold globvar2pred.
-simpl. rewrite H0, H.
-simpl. rewrite emp_sepcon.
-apply derives_refl.
+go_lowerx.
+iIntros "($ & $ & ?)".
+rewrite /globvars2pred /= /globvar2pred /=.
+rewrite H0 H /= bi.emp_sep //.
+Qed.
+
+Lemma finish_process_globvars: 
+ forall E Delta PQR SF c Post,
+  semax E Delta (PQR ∗ SF) c Post ->
+  semax E Delta (PQR ∗ emp ∗ SF) c Post.
+Proof.
+intros.
+rewrite bi.emp_sep; auto.
 Qed.
 
 Definition is_array_type t :=
  match t with Tarray _ _ _ => true | _ => false end.
 
+End mpred.
+
 Ltac process_one_globvar' :=
  first
   [ simple eapply process_globvar_extern; [reflexivity | reflexivity ]
-  | match goal with |- ENTAIL ?Delta, globvars_in_process ?gv _ emp ((?i,?v)::_) |-- _ =>
+  | match goal with |- ENTAIL ?Delta, globvars_in_process ?gv _ emp ((?i,?v)::_) ⊢ _ =>
         (* need this hack because, for some reason, simple eapply does not work here *)
            unify (is_array_type (gvar_info v)) true
      end;
@@ -1544,7 +1350,7 @@ Ltac process_one_globvar' :=
   | simple eapply process_globvar';
       [reflexivity | reflexivity | reflexivity | reflexivity | reflexivity | reflexivity
       | reflexivity | compute; congruence ]
-  | match goal with |- ENTAIL ?Delta, globvars_in_process ?gv _ emp ((?i,?v)::_) |-- _ =>
+  | match goal with |- ENTAIL ?Delta, globvars_in_process ?gv _ emp ((?i,?v)::_) ⊢ _ =>
         (* need this hack because, for some reason, simple eapply does not work here *)
            unify (is_array_type (gvar_info v)) true
      end;
@@ -1553,7 +1359,7 @@ Ltac process_one_globvar' :=
       | compute; clear; congruence
       | repeat eapply map_instantiate; symmetry; apply map_nil
       | compute; split; clear; congruence  ]
-  | match goal with |- ENTAIL ?Delta, globvars_in_process ?gv _ emp ((?i,?v)::_) |-- _ =>
+  | match goal with |- ENTAIL ?Delta, globvars_in_process ?gv _ emp ((?i,?v)::_) ⊢ _ =>
         (* need this hack because, for some reason, simple eapply does not work here *)
            unify (is_array_type (gvar_info v)) true
      end;
@@ -1572,18 +1378,15 @@ Ltac process_one_globvar :=
   eapply ENTAIL_trans; [process_one_globvar' | simpl float_constructor].
 
 Lemma move_globfield_into_done:
- forall Delta gv done S1 R al R',
-  ENTAIL Delta, globvars_in_process gv (S1::done) R al |-- R' ->
-  ENTAIL Delta, globvars_in_process gv done (S1 * R) al |-- R'.
+ forall `{!heapGS Σ} Delta gv done S1 R al R',
+  ENTAIL Delta, globvars_in_process gv (S1::done) R al ⊢ R' ->
+  ENTAIL Delta, globvars_in_process gv done (S1 ∗ R) al ⊢ R'.
 Proof.
 intros.
-eapply ENTAIL_trans; [ | apply H]; clear.
-apply andp_left2.
-unfold globvars_in_process.
-intro rho; simpl; normalize.
-rewrite <- !sepcon_assoc.
-pull_left S1.
-auto.
+rewrite -H.
+apply bi.and_mono; first done.
+unfold globvars_in_process; simpl.
+iIntros "($ & $ & ($ & $) & $)".
 Qed.
 
 (*
@@ -1633,7 +1436,7 @@ Lemma move_globfield_into_SEP0:
  semax Delta (S0 * emp * S3 * S4) c Post.
 Proof.
 intros.
-rewrite sepcon_emp; auto.
+rewrite bi.sep_emp; auto.
 Qed.
 
 *)
@@ -1651,7 +1454,7 @@ Qed.
 Ltac process_idstar :=
      process_one_globvar;
      lazymatch goal with Delta := @abbreviate tycontext _ 
-                             |- ENTAIL _, globvars_in_process _ _ ?A _ |-- _ =>
+                             |- ENTAIL _, globvars_in_process _ _ ?A _ ⊢ _ =>
       match A with id2pred_star _ _ _ (_ ?i) _ =>
          let p := fresh "p" in set (p:=A);
          simpl in p;
@@ -1660,14 +1463,14 @@ Ltac process_idstar :=
          cbv beta iota zeta in p;
          simpl init_data_size in p;
          revert p; rewrite ?offset_offset_val; intro p; simpl Z.add in p;
-         let t := constr:(match (glob_types Delta) ! i with Some x => x | _ => Tvoid end) in
+         let t := constr:(match (glob_types Delta) !! i with Some x => x | _ => Tvoid end) in
          let t := eval hnf in t in
          match t with Tpointer ?t2 _ =>
            repeat match goal with p := ?D |- _ =>
                        match D with context [mapsto ?sh ?t' ?q ?v] =>
                             revert p;
                            change (mapsto sh t' q v) with (mapsto sh size_t q nullval);
-                           rewrite <- (mapsto_size_t_tptr_nullval sh q t2);
+                           rewrite <- (mapsto_tuint_tptr_nullval sh q t2);
                            intro p
                        end end
          | _ => idtac end;
@@ -1676,7 +1479,7 @@ Ltac process_idstar :=
          repeat simple apply move_globfield_into_done
       | _ => idtac
        end
-    | |- ENTAIL _, _ |-- _ => idtac
+    | |- ENTAIL _, _ ⊢ _ => idtac
     end.
 
 Create HintDb zero_val discriminated.
@@ -1728,21 +1531,12 @@ Qed.
 #[export] Hint Rewrite @zero_val_Tlong @zero_val_Tint : zero_val.
 #[export] Hint Rewrite @zero_val_tint @zero_val_tuint @zero_val_tlong @zero_val_tulong @zero_val_tptr : zero_val.
 
-Lemma finish_process_globvars: 
- forall {cs: compspecs}{Espec: OracleKind} Delta PQR SF c Post,
-  semax Delta (PQR * SF) c Post ->
-  semax Delta (PQR * emp * SF) c Post.
-Proof.
-intros.
-rewrite sepcon_emp; auto.
-Qed.
-
 Lemma prog_defs_Clight_mkprogram:
  forall c g p m w,
  prog_defs (Clightdefs.mkprogram c g p m w) = g.
 Proof.
 intros. unfold Clightdefs.mkprogram.
-destruct ( build_composite_env' c w).
+destruct (build_composite_env' c w).
 reflexivity.
 Qed.
 
@@ -1750,13 +1544,13 @@ Ltac process_globals :=
   repeat process_idstar; 
   change (Share.lub extern_retainer _) with Ews;
   change (Share.lub extern_retainer _) with Ers;
-  try change (Vint oo _) with (Vint oo id);
+  try change (Basics.compose Vint _) with (Basics.compose Vint id);
   fold_types;
   rewrite ?Combinators.compose_id_right;
   apply ENTAIL_refl.
 
 Ltac expand_main_pre_old :=
- match goal with | |- semax _ _ (main_pre_old ?prog _ _ * _) _ _ =>
+ match goal with | |- semax _ _ (main_pre_old ?prog _ _ ∗ _) _ _ =>
     rewrite main_pre_start_old;
     unfold prog_vars, prog
                           | |- semax _ _ (main_pre_old ?prog _ _) _ _ =>
@@ -1773,5 +1567,3 @@ simple eapply semax_process_globvars;
  rewrite ?offset_val_unsigned_repr;
  simpl readonly2share;
  autorewrite with zero_val.
-
-
