floyd/proofauto.v
@@ -39,7 +39,7 @@ Require Export VST.floyd.proj_reptype_lemmas.
 Require Export VST.floyd.replace_refill_reptype_lemmas.
 Require Export VST.floyd.sc_set_load_store.
 Require Export VST.floyd.unfold_data_at.
-(* Require Export VST.floyd.globals_lemmas. *)
+Require Export VST.floyd.globals_lemmas.
 Require Export VST.floyd.diagnosis.
 Require Export VST.floyd.freezer.
 Require Export VST.floyd.deadvars.
